\textsl{(2.1)} : y(t) = V_c(t)x(t) = g(x(t))x(t)

%%%%%%%%%%%%%%%%%%%%%%%%%%%%%%%%%%%%%%%%%

\begin{align*}

&\textsl{(2.2)}: SR(s) = \frac{1}{s}H(s) = \frac{\omega_c}{s(s+\omega_c)} \\
&= \frac{A}{s} + \frac{B}{s+\omega_c} = \frac{1}{s} - \frac{1}{s+\omega_c} 

\end{align*}

%%%%%%%%%%%%%%%%%%%%%%%%%%%%%%%%%%%%%%%%%

\textsl{(2.3)}: sr(t) = \mathcal{L}^{-1} \left [ \frac{1}{s} - \frac{1}{s+\omega_c} \right ] 
= (1 - e^{-\omega_ct})u(t)
%%%%%%%%%%%%%%%%%%%%%%%%%%%%%%%%%%%%%%%%%

\textsl{(2.4)} : ctf(x_{dB}) = \left\{\begin{matrix}
x_{dB}, & x_{dB}\leq thrdB\\ 
thrdB+\frac{x_{dB}-thrdB}{ratio},& otherwise
\end{matrix}\right.


%%%%%%%%%%%%%%%%%%%%%%%%%%%%%%%%%%%%%%%%%

\begin{matrix}
\textsl{(3.1)} : H(s) = \frac{Y(s)}{X(s)} = \frac{\omega_c}{\omega_c+s} \\
Y(s) (\omega_c+s) = X(s)\omega_c\\
sY(s) = \omega_c(X(s)-Y(s))\\
\dot{y} = \omega_c(t)(x(t)-y(t))
\end{matrix}

%%%%%%%%%%%%%%%%%%%%%%%%%%%%%%%%%%%%%%%%%%

\textsl{(3.2)} : y(t) = \int_{t}^{t_0}\omega_c(\tau)(x(\tau)-y(\tau))d\tau

%%%%%%%%%%%%%%%%%%%%%%%%%%%%%%%%%%%%%%%%%%

\begin{matrix}
\textsl{(3.3)}: b(x,y) = \left\{\begin{matrix}
w_r,&x<y\\
w_a,& otherwise 

\end{matrix}\right. \\
=(\omega_a-\omega_r)u(x-y)+\omega_r

\end{matrix}


%%%%%%%%%%%%%%%%%%%%%%%%%%%%%%%%%%%%%%%%%%

\textsl{(3.4)}: g(x) = \frac{dB2G(ctf(g2dB(x)))}{x} 

%%%%%%%%%%%%%%%%%%%%%%%%%%%%%%%%%%%%%%%%%

\begin{align*}
&\textsl{(3.5)}: g(x) = \frac{10^{\frac{thrdB + \frac{20log_{10}(x)-thrdB}{ratio}}{20}}}{x}\\
&= \frac{10^{\frac{thrdB}{20}}    10^{\frac{log_{10}(x)}{ratio}} } {x 10^{\frac{thrdB}{20ratio}}}\\
&= \frac{thrlin (x)^{\frac{1}{ratio}}}{x(thrlin)^(\frac{1}{ratio})}\\
&= x^{\frac{1}{ratio}-1}thrlin^{1-\frac{1}{ratio}}\\
&= \frac{x}{thrlin}^{\frac{1}{ratio}-1}
\end{align*}

%%%%%%%%%%%%%%%%%%%%%%%%%%%%%%%%%%%%%%%%%
\textsl{(3.6)}: 
f(x) = 
\left\{\begin{matrix}

1, & x \leq thrlin\\ 
\left (  \frac{x}{thrlin} \right )^{\frac{1}{ratio}-1}, & x > thrlin 

\end{matrix}\right.
%%%%%%%%%%%%%%%%%%%%%%%%%%%%%%%%%%%%%%%%%%
\begin{align*}
 
& \textsl{(4.1)}: \; y = g(x-y)+s, g = \frac{\omega_cT}{2}, y = y_{LP}(t), x = x(t) \\

& \textsl{(4.2)}: \; y = Gx+S, G = \frac{g}{1+g}, S=\frac{s}{1+g} \\

& \textsl{(4.3)}: \; v = g(x-y) = g(x-Gx-S) = g \left(x-\frac{g}{1+g}x-\frac{s}{1+g} \right) \\
& = g\left ( \frac{1}{1+g}x-\frac{s}{1+g} \right ) = g\frac{x-s}{1+g} = G(x-s)

\end{align*} 

%%%%%%%%%%%%%%%%%%%%%%%%%%%%%%%%%%%%%%%%%%
\textsl{(4.4)}:\alpha = e^{-w_cT}

%%%%%%%%%%%%%%%%%%%%%%%%%%%%%%%%%%%%%%%%%%



%%%%%%%%%%%%%%%%%%%%%%%%%%%%%%%%%%%%%%%%%%

\textsl{(5.1)} : y(t) = g(y(t))x(t)

%%%%%%%%%%%%%%%%%%%%%%%%%%%%%%%%%%%%%%%%%%%%

y[n] = \sum_{1}^{n}\frac{x[n-1]+x[n]}{2}T